\documentclass{article}
\input{/home/giannis/Documents/latex/preamble.tex}

\setmainfont{GFS Didot}
\title{Χρήσιμες Ταυτότητες}
\author{tromboni.gd}
\date{}
\DeclareMathOperator{\arcsec}{arcsec}
\DeclareMathOperator{\arccot}{arccot}
\DeclareMathOperator{\arccsc}{arccsc}

\begin{document}
\maketitle
\tableofcontents

\section{Γενικές}
\[
e^{x}=\sum_{n=0}^{\infty}\frac{x^{n}}{n!}
\] 
\[
    \cos x = \sum_{n=0}^{\infty}(-1)^{n}\frac{x^{2n}}{(2n)!}
\]
\[
    \sin x = \sum_{n=0}^{\infty}(-1)^{n}\frac{x^{2n+1}}{(2n+1)!}
\] 
\[
    e^{ix}=\cos x + \mathrm{i} \sin x 
\] 
\[
\cos x = \frac{e^{\mathrm{i}x}+e^{-\mathrm{i}x}}{2} \quad 
\sin x = \frac{e^{\mathrm{i}x}-e^{-\mathrm{i}x}}{2\mathrm{i}}
\] 
\[
    (\cos x + \text{i} \sin x)^{n}=e^{\text{i}nx} = \cos (nx) + \text{i} \sin (nx)
\] 
\[
a^3+b^3+c^3 - 3abc = a^2+b^2+c^2-ab-bc-ca = \frac{1}{2}\left((a-b)^2+(b-c)^2+(c-a)^2\right)
\] 
\[
    (a^2+b^2)(c^2+d^2) = (ac+bd)^2 + (ad-bc)^2
\] 
\section{Τριγωνομετρικές}
\[
    1 = \cos^2x + \sin^2x
\] 
\[
\tan x = \frac{\sin x}{\cos x} \quad \cot x = \frac{\cos x}{\sin x}
\] 
\[
\sec x = \frac{1}{\cos x} \quad \csc x = \frac{1}{\sin x}
\] 
\begin{gather}
    \cos (x+y) = \cos x\cos y - \sin x \sin y \notag\\
    \cos (x-y) = \cos x\cos y + \sin x \sin y \notag\\
    \sin (x+y) = \sin x\cos y + \cos x \sin y \notag\\
    \sin (x-y) = \sin x\cos y - \cos x \sin y \notag
\end{gather}
\begin{gather}
    2\cos x \cos y = \cos (x+y) + \cos (x-y) \notag\\
    2\sin x \cos y = \sin (x+y) - \sin (x-y) \notag\\
    2\sin x \sin y = \cos (x+y) - \cos (x-y) \notag 
\end{gather}
\begin{gather*}
    \cos x + \cos y = 2\cos \left(\frac{x+y}{2}\right)\cos \left(\frac{x-y}{2}\right) \\
    \cos x - \cos y = -2\sin\left(\frac{x+y}{2}\right)\sin \left(\frac{x-y}{2}\right) \\
    \sin x + \sin y = 2\sin \left(\frac{x+y}{2}\right)\cos \left(\frac{x-y}{2}\right) \\
    \sin x - \sin y = 2\sin \left(\frac{x-y}{2}\right)\cos \left(\frac{x+y}{2}\right) 
\end{gather*} 
\begin{gather*}
    \tan (x+y) = \frac{\tan x + \tan y}{1 - \tan x \tan y} \\
    \tan (x-y) = \frac{\tan x - \tan y}{1 + \tan x \tan y} \\
    \cot (x+y) = \frac{\cot x \cot y - 1}{\cot x + \cot y} \\
    \cot (x-y) = \frac{\cot x \cot y + 1}{\cot x - \cot y}
\end{gather*}
\begin{gather*}
    \sin(2x) = 2\sin x\cos x \\
    \cos(2x) = \cos ^2x - \sin ^2x = 2\cos ^2x - 1 = 1 - 2\sin ^2x \\
    2\sin^2x = 1 - \cos(2x) \\
    2\cos^2x = 1 + \cos(2x) 
\end{gather*}
\begin{gather*}
    \sin x = \frac{\tan x}{\sqrt{1+\tan^2 x}} \\
    \cos x = \frac{1}{\sqrt{1+\tan^2 x}}
\end{gather*}
\begin{gather*}
    \tan(2x) = \frac{2\tan x}{1-\tan^2x} \\
    \cot(2x) = \frac{\cot^2x - 1}{2\cot x} \\
    \sin(2x) = \frac{2\tan x}{1 + \tan^2x} \\
    \cos(2x) = \frac{1-\tan^2x}{1+\tan^2x}
\end{gather*}
\begin{gather*}
    \sin(3x) = 3\sin x - 4\sin^3x \\
    \cos(3x) = 4\cos^3x - 3\cos x
\end{gather*}
\begin{gather*}
    (\cos x)' = -\sin x \\
    (\sin x)' = \cos x \\
    (\tan x)' = \sec^2x = 1 + \tan^2x \\
    (\cot x)' = -\csc^2x = -(1 + \cot^2x)
\end{gather*}
\begin{gather*}
    (\arcsin x)' = \frac{1}{\sqrt{1-x^2}} \\
    (\arccos x)' = -\frac{1}{\sqrt{1-x^2}} \\
    (\arctan x)' = \frac{1}{1+x^2} \\
    (\arccot x)' = -\frac{1}{1+x^2} \\
    (\arcsec x)' = \frac{1}{x^2\sqrt{1-\frac{1}{x^2}}} \\
    (\arccsc x)' = -\frac{1}{x^2\sqrt{1-\frac{1}{x^2}}} 
\end{gather*}
\begin{gather*}
    \sin(\arccos x) = \cos(\arcsin x) = \sqrt{1-x^2} \\
    \tan(\arcsin x) = \frac{x}{\sqrt{1-x^2}} \\
    \tan(\arccos x) = \frac{\sqrt{1-x^2}}{x} 
\end{gather*}
\begin{gather}
    
\end{gather}
 
\end{document}
